WIP: Modified heap and value relation generation and added word array proofs
The first change allows users to pass values and types to the heap
relation and value relation generation to either add or ignore those
types and values for the generation.

Proofs for preservation (update and value semantics), correspondence
and upward propagation between the update and value, and
monomorphisation for them length, get and put methods for word arrays
have been added.

Additional proofs about typing, value typing, monomorphisation and
correspondence in general were also added.

cogent/examples/repeat/UpdateSemHelper.thy
@@ -1,8 +1,108 @@
 theory UpdateSemHelper
   imports
     DeterministicRelation3
+    CogentTypingHelper
     Cogent.UpdateSemantics
+    AutoCorres.AutoCorres
 begin
+
+section "Value typing elimination rules"
+
+inductive_cases (in update_sem) u_t_tfunE: "\<Xi>, \<sigma> \<turnstile> u :u TFun a b \<langle>r, w\<rangle>"
+inductive_cases (in update_sem) u_t_tprimE: "\<Xi>, \<sigma> \<turnstile> u :u TPrim t \<langle>r, w\<rangle>"
+inductive_cases (in update_sem) u_t_tconE: "\<Xi>, \<sigma> \<turnstile> u :u TCon n ts s \<langle>r, w\<rangle>"
+inductive_cases (in update_sem) u_t_tunitE: "\<Xi>, \<sigma> \<turnstile> u :u TUnit \<langle>r, w\<rangle>"
+inductive_cases (in update_sem) u_t_tsumE: "\<Xi>, \<sigma> \<turnstile> u :u TSum a \<langle>r, w\<rangle>"
+inductive_cases (in update_sem) u_t_trecordE: "\<Xi>, \<sigma> \<turnstile> u :u TRecord ts s \<langle>r, w\<rangle>"
+inductive_cases (in update_sem) u_t_tproductE: "\<Xi>, \<sigma> \<turnstile> u :u TProduct a b \<langle>r, w\<rangle>"
+
+inductive_cases (in update_sem) u_t_r_temptyE : "\<Xi>', \<sigma> \<turnstile>* fs :ur [] \<langle>r, w\<rangle>"
+
+lemma (in update_sem) uval_typing_record_length:
+assumes "\<Xi>, \<sigma>  \<turnstile>* fs :ur \<tau>s \<langle>r, w\<rangle>"
+shows   "length fs = length \<tau>s"
+using assms proof (induct fs arbitrary: \<tau>s r w)
+qed (auto)
+
+
+lemma (in update_sem) uval_typing_record_alt1:
+  "\<Xi>', \<sigma> \<turnstile>* fs :ur ts \<langle>r, w\<rangle> \<Longrightarrow> 
+      r \<inter> w = {} \<and> length fs = length ts \<and>
+      (\<exists>rs ws. r = \<Union>(set rs) \<and> w = \<Union>(set ws) \<and> length rs = length fs \<and> length ws = length fs \<and>
+        distinct_sets ws \<and>
+        (\<forall>i<length fs. 
+          \<exists>x rp n t s. fs ! i = (x, rp) \<and> ts ! i = (n, t, s) \<and> type_repr t = rp \<and>
+            (s = Taken \<longrightarrow> [] \<turnstile> t wellformed \<and> uval_repr x = rp \<and> uval_repr_deep x = rp \<and> rs ! i = {} \<and> ws ! i = {}) \<and>
+            (s = Present \<longrightarrow> \<Xi>', \<sigma> \<turnstile> x :u t \<langle>rs ! i, ws ! i\<rangle>)))"
+  apply (induct fs arbitrary: ts r w)
+   apply clarsimp
+   apply (erule u_t_r_emptyE; clarsimp)
+  apply clarsimp
+  apply (case_tac ts; clarsimp)
+   apply (erule u_t_r_temptyE; clarsimp)
+  apply (rename_tac a b fs r w n t s ts)
+  apply (clarsimp simp: uval_typing_pointers_noalias)
+  apply (frule uval_typing_record_length)
+  apply simp
+  apply (drule_tac x = ts in meta_spec)
+  apply (case_tac s; clarsimp)
+   apply (drule_tac x = r and y = w in meta_spec2)
+   apply (erule u_t_r_consE; clarsimp)
+   apply (rename_tac fs ts t x n rs ws)
+   apply (rule_tac x = "{} # rs" in exI; clarsimp)
+   apply (rule_tac x = "{} # ws" in exI; clarsimp)
+   apply (rename_tac i)
+   apply (case_tac i; clarsimp)
+  apply (erule u_t_r_consE; clarsimp)
+  apply (rename_tac fs x t r w ts r' w' n)
+  apply (drule_tac x = r' and y = w' in meta_spec2; clarsimp)
+  apply (rename_tac rs ws)
+  apply (rule_tac x = "r # rs" in exI; clarsimp)
+  apply (rule_tac x = "w # ws" in exI; clarsimp)
+  apply (rename_tac i)
+  apply (case_tac i; clarsimp)
+  done
+
+lemma (in update_sem) uval_typing_record_alt2:
+  "r \<inter> w = {} \<and> length fs = length ts \<and>
+   (\<exists>rs ws. r = \<Union>(set rs) \<and> w = \<Union>(set ws) \<and> length rs = length fs \<and> length ws = length fs \<and>
+   distinct_sets ws \<and>
+   (\<forall>i<length fs. 
+      \<exists>x rp n t s. fs ! i = (x, rp) \<and> ts ! i = (n, t, s) \<and> type_repr t = rp \<and>
+          (s = Taken \<longrightarrow> [] \<turnstile> t wellformed \<and> uval_repr x = rp \<and> uval_repr_deep x = rp \<and> rs ! i = {} \<and> ws ! i = {}) \<and>
+          (s = Present \<longrightarrow> \<Xi>', \<sigma> \<turnstile> x :u t \<langle>rs ! i, ws ! i\<rangle>)))
+    \<Longrightarrow> \<Xi>', \<sigma> \<turnstile>* fs :ur ts \<langle>r, w\<rangle>"
+  apply (induct fs arbitrary: ts r w; clarsimp)
+   apply (rule u_t_r_empty)
+  apply (rename_tac a b fs ts rs ws)
+  apply (case_tac ts; clarsimp)
+  apply (rename_tac n t s ts)
+  apply (drule_tac x = ts in meta_spec; clarsimp)
+  apply (drule_tac x = " \<Union> (set (tl rs))" and y = " \<Union> (set (tl ws))" in meta_spec2)
+  apply (erule meta_impE)
+   apply (rule conjI)
+    apply (erule_tac x = 0 in allE; clarsimp)
+    apply (case_tac rs; clarsimp; case_tac ws; clarsimp)
+    apply blast 
+   apply (rule exI, rule conjI, simp)
+   apply (rule exI, rule conjI, simp)
+   apply (rule conjI; clarsimp)
+   apply (rule conjI)
+    apply (erule_tac x = 0 in allE; clarsimp)
+    apply (case_tac ws; clarsimp)
+    apply clarsimp
+    apply (rename_tac i)
+    apply (erule_tac x = "Suc i" in allE; clarsimp)
+    apply (rule conjI; clarsimp simp: nth_tl)
+   apply (frule_tac x = 0 in allE; simp?; clarsimp)
+  apply (case_tac s; clarsimp)
+   apply (rule u_t_r_cons2; simp?)
+   apply (case_tac rs; clarsimp; case_tac ws; clarsimp)
+  apply (case_tac rs; clarsimp; case_tac ws; clarsimp)
+  apply (rule u_t_r_cons1; simp?)
+   apply blast
+  apply blast
+  done
 
 section "Function checking and extraction"
 
@@ -18,12 +118,108 @@ fun uvalfun_to_expr
 "uvalfun_to_expr (UAFunction f ts) = AFun f ts" |
 "uvalfun_to_expr _ = undefined"
 
-inductive_cases (in update_sem) u_t_tfunE: "\<Xi>, \<sigma> \<turnstile> u :u TFun a b \<langle>r, w\<rangle>"
-
 lemma (in update_sem) uval_typing_uvalfun:
   "\<Xi>, \<sigma> \<turnstile> u :u TFun a b \<langle>r, w\<rangle> \<Longrightarrow> is_uvalfun u"
   apply (erule u_t_tfunE; clarsimp)
   done
+
+fun no_rfun
+  where
+"no_rfun (RPrim _) = True" |
+"no_rfun RUnit = True" |
+"no_rfun RFun = False" |
+"no_rfun (RCon n rs) = (find (\<lambda>x. \<not>x) (map no_rfun rs) = option.None)" |
+"no_rfun (RProduct a b) = (if no_rfun a then no_rfun b else False)" |
+"no_rfun (RSum a) = (find (\<lambda>x. \<not>x) (map (no_rfun \<circ> prod.snd) a) = option.None)" |
+"no_rfun (RRecord a) = (find (\<lambda>x. \<not>x) (map no_rfun a) = option.None)" |
+"no_rfun (RPtr a) = no_rfun a"
+
+
+lemma no_tfun_no_rfun:
+  "no_tvars t \<Longrightarrow> no_tfun t \<longleftrightarrow> no_rfun (type_repr t)"
+  apply (induct t; clarsimp simp: find_None_iff_nth list_eq_iff_nth_eq split: if_splits)
+    apply (rename_tac n ts s)
+    apply (case_tac s; clarsimp simp: find_None_iff_nth)
+   apply (rule iffI; clarsimp)
+    apply (rename_tac x i)
+    apply (erule_tac x = i in allE; clarsimp)+
+    apply (clarsimp simp: set_conv_nth)
+    apply (elim meta_allE meta_impE; simp?)
+     apply (intro exI conjI; simp?)
+    apply simp
+   apply (rename_tac x i a aa b)
+   apply (erule_tac x = i in allE; clarsimp)+
+   apply (clarsimp simp: set_conv_nth)
+   apply (elim meta_allE meta_impE; simp?)
+    apply (intro exI conjI; simp?)
+   apply simp
+  apply (rename_tac fs s)
+  apply (case_tac s; clarsimp simp: find_None_iff_nth)
+   apply (rule iffI; clarsimp)
+    apply (rename_tac i)
+    apply (erule_tac x = i in allE; clarsimp)+
+    apply (clarsimp simp: set_conv_nth)
+    apply (elim meta_allE meta_impE; simp?)
+     apply (intro exI conjI; simp?)
+    apply simp
+   apply (rename_tac x i a aa b)
+   apply (erule_tac x = i in allE; clarsimp)+
+   apply (clarsimp simp: set_conv_nth)
+   apply (elim meta_allE meta_impE; simp?)
+    apply (intro exI conjI; simp?)
+   apply simp
+  apply (rule iffI; clarsimp)
+   apply (rename_tac i)
+   apply (erule_tac x = i in allE; clarsimp)+
+   apply (clarsimp simp: set_conv_nth)
+   apply (elim meta_allE meta_impE; simp?)
+    apply (intro exI conjI; simp?)
+   apply simp
+  apply (rename_tac x i a aa b)
+  apply (erule_tac x = i in allE; clarsimp)+
+  apply (clarsimp simp: set_conv_nth)
+  apply (elim meta_allE meta_impE; simp?)
+   apply (intro exI conjI; simp?)
+  apply simp
+  done
+
+fun no_ufun
+  where
+"no_ufun (UPrim _) = True" |
+"no_ufun UUnit  = True" |
+"no_ufun (USum a b r) = no_ufun b" |
+"no_ufun (UAbstract _) = True" |
+"no_ufun (UFunction _ _) = False" |
+"no_ufun (UAFunction _ _) = False" |
+"no_ufun (UProduct a b) = (if no_ufun a then no_ufun b else False)" |
+"no_ufun (URecord xs) = (find (\<lambda>x. \<not>x) (map (no_ufun \<circ> prod.fst) xs) = option.None)" |
+"no_ufun (UPtr _ r) = no_rfun r"
+
+
+lemma (in update_sem) no_tfun_imp_no_vfuns:
+  "\<lbrakk>no_tvars t; no_tfun t; no_taken t; no_tcon t;  \<Xi>,  \<sigma> \<turnstile> v :u t \<langle>r, w\<rangle>\<rbrakk> \<Longrightarrow> no_ufun v"
+proof (induct t arbitrary: \<sigma> v r w)
+  case (TRecord x1a x2a)
+  then show ?case 
+    apply (clarsimp simp: find_None_iff_nth  split: if_splits)
+    apply (erule u_t_trecordE; clarsimp simp: find_None_iff_nth)
+      apply (frule uval_typing_record_length)
+      apply (rename_tac fs i)
+      apply (erule_tac x = i in allE; clarsimp)+
+      apply (clarsimp simp: set_conv_nth)
+      apply (rename_tac fs i x a b)
+      apply (case_tac b; clarsimp)
+      apply (drule (2) uval_typing_record_nth'; clarsimp)
+      apply (elim meta_allE meta_impE; assumption?; simp?)
+      apply (intro exI conjI; simp?)
+     apply (rename_tac fs r l ptrl i)
+     apply (erule_tac x = i in allE; clarsimp)+
+     apply (clarsimp simp: no_tfun_no_rfun)
+    apply (rename_tac fs w l ptrl i)
+    apply (erule_tac x = i in allE; clarsimp)+
+    apply (clarsimp simp: no_tfun_no_rfun)
+    done
+qed (fastforce simp: find_None_iff elim: u_t_tunitE u_t_tprimE u_t_tconE u_t_sumE u_t_tproductE)+
 
 section "Evaluation elimination rules"
 
@@ -307,6 +503,19 @@ lemma frame_empty:
   apply (clarsimp simp: frame_def fun_eq_iff)
   done
 
+lemma frame_expand:
+  "\<lbrakk>frame \<sigma> w \<sigma>' w'; \<sigma> p \<noteq> option.None\<rbrakk> \<Longrightarrow> frame \<sigma> (insert p w) \<sigma>' (insert p w')"
+  "\<lbrakk>frame \<sigma> w \<sigma>' w'; \<forall>p\<in>s. \<sigma> p \<noteq> option.None\<rbrakk> \<Longrightarrow> frame \<sigma> (s \<union> w) \<sigma>' (s \<union> w')"
+   apply (clarsimp simp: frame_def)
+   apply (rule conjI; clarsimp)
+  apply (clarsimp simp: frame_def)
+  apply (rule conjI; clarsimp)
+  done
+
+lemma frame_single_update_expand:
+  "l \<in> w \<Longrightarrow> frame \<sigma> w (\<sigma>(l \<mapsto> v)) w"
+  by (clarsimp simp: frame_def)
+
 lemma discardable_or_shareable_not_writable:
 assumes "D \<in> k \<or> S \<in> k"
 shows "\<lbrakk> \<Xi>', \<sigma> \<turnstile>  v  :u  \<tau>  \<langle> r , w \<rangle>; K' \<turnstile>  \<tau>  :\<kappa>  k \<rbrakk> \<Longrightarrow> w = {}"
@@ -336,6 +545,15 @@ and   "\<lbrakk> \<Xi>', \<sigma> \<turnstile>* fs :ur map (\<lambda>(n, t, b). 
   apply (clarsimp split: record_state.splits)
   apply (rename_tac a aa ab ac)
   apply (cut_tac K = "[]" and t = ac in bang_kinding_fn; clarsimp)
+  done
+
+lemma no_heap_no_pointers:
+  "\<lbrakk>no_tvars t; no_theap t; \<Xi>', \<sigma> \<turnstile> v :u t \<langle>r, w\<rangle>\<rbrakk> \<Longrightarrow> r = {} \<and> w = {}"
+  apply (frule uval_typing_to_wellformed)
+  apply (cut_tac K = "[]" and t= t in  no_heap_all_kind; simp?)
+  apply (frule_tac k = UNIV in escapable_no_readers(1); simp?)
+  apply (frule  discardable_or_shareable_not_writable(1)[rotated 1]; simp?)
+  apply blast
   done
 
 end (* of context *)
